Constructions file

VCVio/OracleComp/SimSemantics/Simulate.lean
@@ -44,9 +44,6 @@ def simulate' (so : spec₁ →[σ]ₛₒ spec₂) (oa : OracleComp spec₁ α) 
     OracleComp spec₂ α :=
   fst <$> simulate so oa s
 
--- lemma simulate'.def (so : spec₁ →[σ]ₛₒ spec₂) (oa : OracleComp spec₁ α) (s : σ) :
---     simulate' so oa s = fst <$> simulate so oa s := rfl
-
 namespace OracleComp
 
 variable {spec₁ spec₂ : OracleSpec} {α β γ σ : Type}
@@ -123,80 +120,3 @@ lemma support_simulate'_subset_support (oa : OracleComp spec₁ α) (s : σ) :
 end support
 
 end OracleComp
-
-namespace SimOracle
-
-section append
-
-/-- Given simulation oracles `so` and `so'` with source oracles `spec₁` and `spec₂` respectively,
-with the same target oracles `specₜ`, construct a new simulation oracle from `specₜ`,
-answering queries to either oracle set with queries to the corresponding simulation oracle. -/
-def append (so : spec₁ →[σ]ₛₒ specₜ) (so' : spec₂ →[τ]ₛₒ specₜ) :
-    spec₁ ++ spec₂ →[σ × τ]ₛₒ specₜ :=
-  λ i ↦ match i with
-  | (inl i) => λ ⟨t, s₁, s₂⟩ ↦ do
-      let ⟨u, s₁'⟩ ← so i (t, s₁) return (u, s₁', s₂)
-  | (inr i) => λ ⟨t, s₁, s₂⟩ ↦ do
-      let ⟨u, s₂'⟩ ← so' i (t, s₂) return (u, s₁, s₂')
-
-infixl : 65 " ++ₛₒ " => append
-
-end append
-
-section compose
-
-/-- Given a simulation oracle `so` from `spec₁` to `spec₂` and a simulation oracle `so'` from
-`spec₂` to a final target set of oracles `specₜ`, construct a new simulation oracle
-from `spec₁` to `spec₂` by first substituting queries using `so`, and then further
-substituting with the oracles in `so'`. -/
-def compose (so : spec₁ →[σ]ₛₒ spec₂) (so' : spec₂ →[τ]ₛₒ specₜ) :
-    spec₁ →[σ × τ]ₛₒ specₜ :=
-  λ i ⟨t, s₁, s₂⟩ ↦ (λ ⟨⟨t, s₁⟩, s₂⟩ ↦ ⟨t, s₁, s₂⟩) <$>
-    simulate so' (so i (t, s₁)) s₂
-
-infixl : 65 " ∘ₛₒ " => λ so' so ↦ compose so so'
-
-end compose
-
-section maskState
-
--- TODO
-
-end maskState
-
-end SimOracle
-
-/-- "Simulate" a computation using the original oracles by "replacing" queries with queries.
-This operates as an actual identity for `simulate'`, in that we get an exact equality
-between the new and original computation.
-
-This can be useful especially with `SimOracle.append`, in order to simulate a single oracle
-in a larger set of oracles, leaving the behavior of other oracles unchanged.
-
-This is importantly different than `unifOracle`, which preserves probabilities but
-changes the target oracle spec to `unifSpec` by explicitly choosing outputs randomly. -/
-def idOracle (spec : OracleSpec) : spec →ₛₒ spec :=
-  λ i ⟨t, ()⟩ ↦ ((., ())) <$> query i t
-
-namespace idOracle
-
-variable (spec : OracleSpec)
-
-@[simp]
-lemma apply_eq : idOracle spec i = λ ⟨t, ()⟩ ↦ ((., ())) <$> query i t := rfl
-
-@[simp]
-lemma simulate_eq (oa : OracleComp spec α) (s : Unit) :
-    simulate (idOracle _) oa s = ((·, ())) <$> oa := by
-  revert s
-  induction oa using OracleComp.inductionOn with
-  | h_pure x => exact λ _ ↦ rfl
-  | h_query_bind i t oa hoa =>
-      exact λ () ↦ by simp [map_eq_bind_pure_comp, hoa]
-
-@[simp]
-lemma simulate'_eq (oa : OracleComp spec α) (s : Unit) :
-    simulate' (idOracle _) oa s = oa := by
-  simp [simulate', Functor.map_map, Function.comp]
-
-end idOracle
