VCVio/OracleComp/SimSemantics/Constructions.lean
@@ -1,0 +1,120 @@
+/-
+Copyright (c) 2024 Devon Tuma. All rights reserved.
+Released under Apache 2.0 license as described in the file LICENSE.
+Authors: Devon Tuma
+-/
+import VCVio.OracleComp.SimSemantics.Simulate
+
+/-!
+# Basic Constructions of Simulation Oracles
+
+This file defines a number of basic simulation oracles, as well as operations to combine them.
+-/
+
+open OracleSpec OracleComp Prod Sum
+
+namespace SimOracle
+
+section append
+
+variable {spec₁ spec₂ specₜ : OracleSpec} {σ τ : Type}
+
+/-- Given simulation oracles `so` and `so'` with source oracles `spec₁` and `spec₂` respectively,
+with the same target oracles `specₜ`, construct a new simulation oracle from `specₜ`,
+answering queries to either oracle set with queries to the corresponding simulation oracle. -/
+def append (so : spec₁ →[σ]ₛₒ specₜ) (so' : spec₂ →[τ]ₛₒ specₜ) :
+    spec₁ ++ spec₂ →[σ × τ]ₛₒ specₜ :=
+  λ i ↦ match i with
+  | (inl i) => λ ⟨t, s₁, s₂⟩ ↦ do
+      let ⟨u, s₁'⟩ ← so i (t, s₁) return (u, s₁', s₂)
+  | (inr i) => λ ⟨t, s₁, s₂⟩ ↦ do
+      let ⟨u, s₂'⟩ ← so' i (t, s₂) return (u, s₁, s₂')
+
+infixl : 65 " ++ₛₒ " => append
+
+@[simp]
+lemma append_apply_inl (so : spec₁ →[σ]ₛₒ specₜ) (so' : spec₂ →[τ]ₛₒ specₜ)
+  (i : spec₁.ι) : (so ++ₛₒ so') (inl i) = λ ⟨t, s₁, s₂⟩ ↦ do
+      let ⟨u, s₁'⟩ ← so i (t, s₁) return (u, s₁', s₂) := rfl
+
+@[simp]
+lemma append_apply_inr (so : spec₁ →[σ]ₛₒ specₜ) (so' : spec₂ →[τ]ₛₒ specₜ)
+  (i : spec₂.ι) : (so ++ₛₒ so') (inr i) = λ ⟨t, s₁, s₂⟩ ↦ do
+      let ⟨u, s₂'⟩ ← so' i (t, s₂) return (u, s₁, s₂') := rfl
+
+end append
+
+section compose
+
+variable {spec₁ spec₂ specₜ : OracleSpec} {σ τ : Type}
+
+/-- Given a simulation oracle `so` from `spec₁` to `spec₂` and a simulation oracle `so'` from
+`spec₂` to a final target set of oracles `specₜ`, construct a new simulation oracle
+from `spec₁` to `spec₂` by first substituting queries using `so`, and then further
+substituting with the oracles in `so'`. -/
+def compose (so : spec₁ →[σ]ₛₒ spec₂) (so' : spec₂ →[τ]ₛₒ specₜ) :
+    spec₁ →[σ × τ]ₛₒ specₜ :=
+  λ i ⟨t, s₁, s₂⟩ ↦ (λ ⟨⟨t, s₁⟩, s₂⟩ ↦ ⟨t, s₁, s₂⟩) <$>
+    simulate so' (so i (t, s₁)) s₂
+
+infixl : 65 " ∘ₛₒ " => λ so' so ↦ compose so so'
+
+@[simp]
+lemma compose_apply (so : spec₁ →[σ]ₛₒ spec₂) (so' : spec₂ →[τ]ₛₒ specₜ)
+  (i : spec₁.ι) : (so' ∘ₛₒ so) i = λ ⟨t, s₁, s₂⟩ ↦ (λ ⟨⟨t, s₁⟩, s₂⟩ ↦ ⟨t, s₁, s₂⟩) <$>
+    simulate so' (so i (t, s₁)) s₂ := rfl
+
+end compose
+
+variable {spec specₜ : OracleSpec} {σ τ : Type}
+
+section maskState
+
+/-- Substitute an equivalent type for the state of a simulation oracle, by using the equivalence
+to move back and forth between the states as needed.
+This can be useful when operations such like `simOracle.append` add on a state of type `Unit`.-/
+def maskState (so : spec →[σ]ₛₒ specₜ) (e : σ ≃ τ) : spec →[τ]ₛₒ specₜ :=
+  λ i ⟨t, s⟩ ↦ map id e <$> so i (t, e.symm s)
+
+@[simp]
+lemma maskState_apply (so : spec →[σ]ₛₒ specₜ) (e : σ ≃ τ) (i : spec.ι) :
+  so.maskState e i = λ ⟨t, s⟩ ↦ map id e <$> so i (t, e.symm s) := rfl
+
+end maskState
+
+end SimOracle
+
+/-- "Simulate" a computation using the original oracles by "replacing" queries with queries.
+This operates as an actual identity for `simulate'`, in that we get an exact equality
+between the new and original computation.
+
+This can be useful especially with `SimOracle.append`, in order to simulate a single oracle
+in a larger set of oracles, leaving the behavior of other oracles unchanged.
+
+This is importantly different than `unifOracle`, which preserves probabilities but
+changes the target oracle spec to `unifSpec` by explicitly choosing outputs randomly. -/
+def idOracle (spec : OracleSpec) : spec →ₛₒ spec :=
+  λ i ⟨t, ()⟩ ↦ ((., ())) <$> query i t
+
+namespace idOracle
+
+variable (spec : OracleSpec)
+
+@[simp]
+lemma apply_eq : idOracle spec i = λ ⟨t, ()⟩ ↦ ((., ())) <$> query i t := rfl
+
+@[simp]
+lemma simulate_eq (oa : OracleComp spec α) (s : Unit) :
+    simulate (idOracle _) oa s = ((·, ())) <$> oa := by
+  revert s
+  induction oa using OracleComp.inductionOn with
+  | h_pure x => exact λ _ ↦ rfl
+  | h_query_bind i t oa hoa =>
+      exact λ () ↦ by simp [map_eq_bind_pure_comp, hoa]
+
+@[simp]
+lemma simulate'_eq (oa : OracleComp spec α) (s : Unit) :
+    simulate' (idOracle _) oa s = oa := by
+  simp [simulate', Functor.map_map, Function.comp]
+
+end idOracle
